Instances/ISAs/VexConcrete.lean
@@ -31,6 +31,8 @@ def evalAmd64CalculateConditionZero
 @[simp] def evalCond {Reg : Type} [DecidableEq Reg] [Fintype Reg]
     (state : ConcreteState Reg) (temps : TempEnv) : Cond Reg → Bool
   | .eq64 lhs rhs => evalExpr state temps lhs == evalExpr state temps rhs
+  | .lt64 lhs rhs => decide (evalExpr state temps lhs < evalExpr state temps rhs)
+  | .le64 lhs rhs => decide (evalExpr state temps lhs ≤ evalExpr state temps rhs)
   | .amd64CalculateCondition code ccOp ccDep1 ccDep2 ccNdep =>
       if code = 0x4 then
         evalAmd64CalculateConditionZero
